<?xml version="1.0"?>
<rdf:RDF xmlns="http://www.semanticweb.org/mguen/ontologies/2024/1/MiTO#"
     xml:base="http://www.semanticweb.org/mguen/ontologies/2024/1/MiTO"
     xmlns:dc="http://purl.org/dc/elements/1.1/"
     xmlns:owl="http://www.w3.org/2002/07/owl#"
     xmlns:rdf="http://www.w3.org/1999/02/22-rdf-syntax-ns#"
     xmlns:xml="http://www.w3.org/XML/1998/namespace"
     xmlns:xsd="http://www.w3.org/2001/XMLSchema#"
     xmlns:mito="https://github.com/matteo-guenci/MiTO/blob/main/MiTO_Ontology/MiTO_Samod_it_1.owl#"
     xmlns:rdfs="http://www.w3.org/2000/01/rdf-schema#">
    <owl:Ontology rdf:about="https://github.com/matteo-guenci/MiTO/blob/main/MiTO_Ontology/MiTO_Samod_it_1.owl"/>
    


    <!-- 
    ///////////////////////////////////////////////////////////////////////////////////////
    //
    // Annotation properties
    //
    ///////////////////////////////////////////////////////////////////////////////////////
     -->

    


    <!-- http://purl.org/dc/elements/1.1/description -->

    <owl:AnnotationProperty rdf:about="http://purl.org/dc/elements/1.1/description"/>
    


    <!-- 
    ///////////////////////////////////////////////////////////////////////////////////////
    //
    // Object Properties
    //
    ///////////////////////////////////////////////////////////////////////////////////////
     -->

    


    <!-- https://github.com/matteo-guenci/MiTO/blob/main/MiTO_Ontology/MiTO_Samod_it_1.owl#hasMentionType -->

    <owl:ObjectProperty rdf:about="https://github.com/matteo-guenci/MiTO/blob/main/MiTO_Ontology/MiTO_Samod_it_1.owl#hasMentionType">
        <rdfs:domain rdf:resource="https://github.com/matteo-guenci/MiTO/blob/main/MiTO_Ontology/MiTO_Samod_it_1.owl#Mention"/>
        <rdfs:range rdf:resource="https://github.com/matteo-guenci/MiTO/blob/main/MiTO_Ontology/MiTO_Samod_it_1.owl#MentionType"/>
        <rdfs:comment xml:lang="en">A data property that aims to define the implicit or explicit character of the mention it is describing</rdfs:comment>
    </owl:ObjectProperty>
    


    <!-- https://github.com/matteo-guenci/MiTO/blob/main/MiTO_Ontology/MiTO_Samod_it_1.owl#hasMentionedEntity -->

    <owl:ObjectProperty rdf:about="https://github.com/matteo-guenci/MiTO/blob/main/MiTO_Ontology/MiTO_Samod_it_1.owl#hasMentionedEntity">
        <rdfs:domain rdf:resource="https://github.com/matteo-guenci/MiTO/blob/main/MiTO_Ontology/MiTO_Samod_it_1.owl#Mention"/>
        <rdfs:range>
            <owl:Class>
                <owl:unionOf rdf:parseType="Collection">
                    <rdf:Description rdf:about="https://github.com/matteo-guenci/MiTO/blob/main/MiTO_Ontology/MiTO_Samod_it_1.owl#Person"/>
                    <rdf:Description rdf:about="https://github.com/matteo-guenci/MiTO/blob/main/MiTO_Ontology/MiTO_Samod_it_1.owl#Thing"/>
                </owl:unionOf>
            </owl:Class>
        </rdfs:range>
        <rdfs:comment xml:lang="en">A property that relates the mention to the mentioned entity.</rdfs:comment>
    </owl:ObjectProperty>
    


    <!-- https://github.com/matteo-guenci/MiTO/blob/main/MiTO_Ontology/MiTO_Samod_it_1.owl#hasMentioningEntity -->

    <owl:ObjectProperty rdf:about="https://github.com/matteo-guenci/MiTO/blob/main/MiTO_Ontology/MiTO_Samod_it_1.owl#hasMentioningEntity">
        <rdfs:domain rdf:resource="https://github.com/matteo-guenci/MiTO/blob/main/MiTO_Ontology/MiTO_Samod_it_1.owl#Mention"/>
        <rdfs:range rdf:resource="https://github.com/matteo-guenci/MiTO/blob/main/MiTO_Ontology/MiTO_Samod_it_1.owl#Article"/>
        <rdfs:comment xml:lang="en">A property that relates the mention to the mentioning entity.</rdfs:comment>
    </owl:ObjectProperty>
    


    <!-- https://github.com/matteo-guenci/MiTO/blob/main/MiTO_Ontology/MiTO_Samod_it_1.owl#mentions -->

    <owl:ObjectProperty rdf:about="https://github.com/matteo-guenci/MiTO/blob/main/MiTO_Ontology/MiTO_Samod_it_1.owl#mentions">
        <rdfs:comment xml:lang="en">The mentioning entity mentions the mentioned entity, either directly and explicitly (when the mention is clearly stated: &quot;... those reasons brought me to think that the best soulution could be the application of SoftwareX ...&quot;), indirectly (e.g.  when a publication mentions a method or algorithm without explicitly naming the software that implements it), or implicitly (e.g.when a publication uses certain terminology or conventions that are specific to a software without directly mentioning the software).</rdfs:comment>
    </owl:ObjectProperty>
    


    <!-- 
    ///////////////////////////////////////////////////////////////////////////////////////
    //
    // Classes
    //
    ///////////////////////////////////////////////////////////////////////////////////////
     -->

    


    <!-- https://github.com/matteo-guenci/MiTO/blob/main/MiTO_Ontology/MiTO_Samod_it_1.owl#Article -->

    <owl:Class rdf:about="https://github.com/matteo-guenci/MiTO/blob/main/MiTO_Ontology/MiTO_Samod_it_1.owl#Article">
        <rdfs:comment xml:lang="en">The realization of a piece of writing on a particular topic, usually published within a periodical publication (e.g. journal, magazine and newspaper).</rdfs:comment>
    </owl:Class>
    


    <!-- https://github.com/matteo-guenci/MiTO/blob/main/MiTO_Ontology/MiTO_Samod_it_1.owl#Mention -->

    <owl:Class rdf:about="https://github.com/matteo-guenci/MiTO/blob/main/MiTO_Ontology/MiTO_Samod_it_1.owl#Mention">
        <rdfs:comment xml:lang="en">Originally: the action of calling to mind or commemorating something in speech or writing. Subsequently in more restricted sense: the action or an act of referring to, remarking upon, or introducing the name of a person or thing in spoken or written discourse, often incidentally and as not necessarily essential to the discussion.
Stated by https://www.oed.com/dictionary/mention_n?tl=true</rdfs:comment>
    </owl:Class>
    


    <!-- https://github.com/matteo-guenci/MiTO/blob/main/MiTO_Ontology/MiTO_Samod_it_1.owl#MentionType -->

    <owl:Class rdf:about="https://github.com/matteo-guenci/MiTO/blob/main/MiTO_Ontology/MiTO_Samod_it_1.owl#MentionType">
        <rdfs:comment xml:lang="en">The aim of this class is to reify the implicit or explicit characteristic of a mention.</rdfs:comment>
    </owl:Class>
    


    <!-- https://github.com/matteo-guenci/MiTO/blob/main/MiTO_Ontology/MiTO_Samod_it_1.owl#Person -->

    <owl:Class rdf:about="https://github.com/matteo-guenci/MiTO/blob/main/MiTO_Ontology/MiTO_Samod_it_1.owl#Person">
        <rdfs:comment xml:lang="en">An individual. The entity defined as person encompasses individuals that are deceased as well as those that are living.</rdfs:comment>
    </owl:Class>
    


    <!-- https://github.com/matteo-guenci/MiTO/blob/main/MiTO_Ontology/MiTO_Samod_it_1.owl#Thing -->

    <owl:Class rdf:about="https://github.com/matteo-guenci/MiTO/blob/main/MiTO_Ontology/MiTO_Samod_it_1.owl#Thing">
        <rdfs:comment xml:lang="en">This class identify simply everything that could be mentioned that is not a Person (e.g. Softwares, Datasets, Workflows, Methodologies...)</rdfs:comment>
    </owl:Class>
    


    <!-- 
    ///////////////////////////////////////////////////////////////////////////////////////
    //
    // Individuals
    //
    ///////////////////////////////////////////////////////////////////////////////////////
     -->

    


    <!-- https://github.com/matteo-guenci/MiTO/blob/main/MiTO_Ontology/MiTO_Samod_it_1.owl#Article1 -->

    <owl:NamedIndividual rdf:about="https://github.com/matteo-guenci/MiTO/blob/main/MiTO_Ontology/MiTO_Samod_it_1.owl#Article1">
        <rdf:type rdf:resource="https://github.com/matteo-guenci/MiTO/blob/main/MiTO_Ontology/MiTO_Samod_it_1.owl#Article"/>
        <mito:mentions rdf:resource="https://github.com/matteo-guenci/MiTO/blob/main/MiTO_Ontology/MiTO_Samod_it_1.owl#Dataset1"/>
        <mito:mentions rdf:resource="https://github.com/matteo-guenci/MiTO/blob/main/MiTO_Ontology/MiTO_Samod_it_1.owl#Methodology1"/>
        <mito:mentions rdf:resource="https://github.com/matteo-guenci/MiTO/blob/main/MiTO_Ontology/MiTO_Samod_it_1.owl#Person1"/>
        <mito:mentions rdf:resource="https://github.com/matteo-guenci/MiTO/blob/main/MiTO_Ontology/MiTO_Samod_it_1.owl#Software1"/>
    </owl:NamedIndividual>
    


    <!-- https://github.com/matteo-guenci/MiTO/blob/main/MiTO_Ontology/MiTO_Samod_it_1.owl#Dataset1 -->

    <owl:NamedIndividual rdf:about="https://github.com/matteo-guenci/MiTO/blob/main/MiTO_Ontology/MiTO_Samod_it_1.owl#Dataset1">
        <rdf:type rdf:resource="https://github.com/matteo-guenci/MiTO/blob/main/MiTO_Ontology/MiTO_Samod_it_1.owl#Thing"/>
    </owl:NamedIndividual>
    


    <!-- https://github.com/matteo-guenci/MiTO/blob/main/MiTO_Ontology/MiTO_Samod_it_1.owl#ExplicitMention -->

    <owl:NamedIndividual rdf:about="https://github.com/matteo-guenci/MiTO/blob/main/MiTO_Ontology/MiTO_Samod_it_1.owl#ExplicitMention">
        <rdf:type rdf:resource="https://github.com/matteo-guenci/MiTO/blob/main/MiTO_Ontology/MiTO_Samod_it_1.owl#MentionType"/>
    </owl:NamedIndividual>
    


    <!-- https://github.com/matteo-guenci/MiTO/blob/main/MiTO_Ontology/MiTO_Samod_it_1.owl#ImplicitMention -->

    <owl:NamedIndividual rdf:about="https://github.com/matteo-guenci/MiTO/blob/main/MiTO_Ontology/MiTO_Samod_it_1.owl#ImplicitMention">
        <rdf:type rdf:resource="https://github.com/matteo-guenci/MiTO/blob/main/MiTO_Ontology/MiTO_Samod_it_1.owl#MentionType"/>
    </owl:NamedIndividual>
    


    <!-- https://github.com/matteo-guenci/MiTO/blob/main/MiTO_Ontology/MiTO_Samod_it_1.owl#Mention1 -->

    <owl:NamedIndividual rdf:about="https://github.com/matteo-guenci/MiTO/blob/main/MiTO_Ontology/MiTO_Samod_it_1.owl#Mention1">
        <rdf:type rdf:resource="https://github.com/matteo-guenci/MiTO/blob/main/MiTO_Ontology/MiTO_Samod_it_1.owl#Mention"/>
        <mito:hasMentionType rdf:resource="https://github.com/matteo-guenci/MiTO/blob/main/MiTO_Ontology/MiTO_Samod_it_1.owl#ExplicitMention"/>
        <mito:hasMentionedEntity rdf:resource="https://github.com/matteo-guenci/MiTO/blob/main/MiTO_Ontology/MiTO_Samod_it_1.owl#Dataset1"/>
        <mito:hasMentioningEntity rdf:resource="https://github.com/matteo-guenci/MiTO/blob/main/MiTO_Ontology/MiTO_Samod_it_1.owl#Article1"/>
    </owl:NamedIndividual>
    


    <!-- https://github.com/matteo-guenci/MiTO/blob/main/MiTO_Ontology/MiTO_Samod_it_1.owl#Mention2 -->

    <owl:NamedIndividual rdf:about="https://github.com/matteo-guenci/MiTO/blob/main/MiTO_Ontology/MiTO_Samod_it_1.owl#Mention2">
        <rdf:type rdf:resource="https://github.com/matteo-guenci/MiTO/blob/main/MiTO_Ontology/MiTO_Samod_it_1.owl#Mention"/>
        <mito:hasMentionType rdf:resource="https://github.com/matteo-guenci/MiTO/blob/main/MiTO_Ontology/MiTO_Samod_it_1.owl#ExplicitMention"/>
        <mito:hasMentionedEntity rdf:resource="https://github.com/matteo-guenci/MiTO/blob/main/MiTO_Ontology/MiTO_Samod_it_1.owl#Methodology1"/>
        <mito:hasMentioningEntity rdf:resource="https://github.com/matteo-guenci/MiTO/blob/main/MiTO_Ontology/MiTO_Samod_it_1.owl#Article1"/>
    </owl:NamedIndividual>
    


    <!-- https://github.com/matteo-guenci/MiTO/blob/main/MiTO_Ontology/MiTO_Samod_it_1.owl#Mention3 -->

    <owl:NamedIndividual rdf:about="https://github.com/matteo-guenci/MiTO/blob/main/MiTO_Ontology/MiTO_Samod_it_1.owl#Mention3">
        <rdf:type rdf:resource="https://github.com/matteo-guenci/MiTO/blob/main/MiTO_Ontology/MiTO_Samod_it_1.owl#Mention"/>
        <mito:hasMentionType rdf:resource="https://github.com/matteo-guenci/MiTO/blob/main/MiTO_Ontology/MiTO_Samod_it_1.owl#ExplicitMention"/>
        <mito:hasMentionedEntity rdf:resource="https://github.com/matteo-guenci/MiTO/blob/main/MiTO_Ontology/MiTO_Samod_it_1.owl#Software1"/>
        <mito:hasMentioningEntity rdf:resource="https://github.com/matteo-guenci/MiTO/blob/main/MiTO_Ontology/MiTO_Samod_it_1.owl#Article1"/>
    </owl:NamedIndividual>
    


    <!-- https://github.com/matteo-guenci/MiTO/blob/main/MiTO_Ontology/MiTO_Samod_it_1.owl#Mention4 -->

    <owl:NamedIndividual rdf:about="https://github.com/matteo-guenci/MiTO/blob/main/MiTO_Ontology/MiTO_Samod_it_1.owl#Mention4">
        <rdf:type rdf:resource="https://github.com/matteo-guenci/MiTO/blob/main/MiTO_Ontology/MiTO_Samod_it_1.owl#Mention"/>
        <mito:hasMentionType rdf:resource="https://github.com/matteo-guenci/MiTO/blob/main/MiTO_Ontology/MiTO_Samod_it_1.owl#ImplicitMention"/>
        <mito:hasMentionedEntity rdf:resource="https://github.com/matteo-guenci/MiTO/blob/main/MiTO_Ontology/MiTO_Samod_it_1.owl#Person1"/>
        <mito:hasMentioningEntity rdf:resource="https://github.com/matteo-guenci/MiTO/blob/main/MiTO_Ontology/MiTO_Samod_it_1.owl#Article1"/>
    </owl:NamedIndividual>
    


    <!-- https://github.com/matteo-guenci/MiTO/blob/main/MiTO_Ontology/MiTO_Samod_it_1.owl#Mention5 -->

    <owl:NamedIndividual rdf:about="https://github.com/matteo-guenci/MiTO/blob/main/MiTO_Ontology/MiTO_Samod_it_1.owl#Mention5">
        <mito:hasMentionType rdf:resource="https://github.com/matteo-guenci/MiTO/blob/main/MiTO_Ontology/MiTO_Samod_it_1.owl#ImplicitMention"/>
        <mito:hasMentionedEntity rdf:resource="https://github.com/matteo-guenci/MiTO/blob/main/MiTO_Ontology/MiTO_Samod_it_1.owl#Theory1"/>
        <mito:hasMentioningEntity rdf:resource="https://github.com/matteo-guenci/MiTO/blob/main/MiTO_Ontology/MiTO_Samod_it_1.owl#Article1"/>
    </owl:NamedIndividual>
    


    <!-- https://github.com/matteo-guenci/MiTO/blob/main/MiTO_Ontology/MiTO_Samod_it_1.owl#Methodology1 -->

    <owl:NamedIndividual rdf:about="https://github.com/matteo-guenci/MiTO/blob/main/MiTO_Ontology/MiTO_Samod_it_1.owl#Methodology1">
        <rdf:type rdf:resource="https://github.com/matteo-guenci/MiTO/blob/main/MiTO_Ontology/MiTO_Samod_it_1.owl#Thing"/>
    </owl:NamedIndividual>
    


    <!-- https://github.com/matteo-guenci/MiTO/blob/main/MiTO_Ontology/MiTO_Samod_it_1.owl#Person1 -->

    <owl:NamedIndividual rdf:about="https://github.com/matteo-guenci/MiTO/blob/main/MiTO_Ontology/MiTO_Samod_it_1.owl#Person1">
        <rdf:type rdf:resource="https://github.com/matteo-guenci/MiTO/blob/main/MiTO_Ontology/MiTO_Samod_it_1.owl#Person"/>
    </owl:NamedIndividual>
    


    <!-- https://github.com/matteo-guenci/MiTO/blob/main/MiTO_Ontology/MiTO_Samod_it_1.owl#Software1 -->

    <owl:NamedIndividual rdf:about="https://github.com/matteo-guenci/MiTO/blob/main/MiTO_Ontology/MiTO_Samod_it_1.owl#Software1">
        <rdf:type rdf:resource="https://github.com/matteo-guenci/MiTO/blob/main/MiTO_Ontology/MiTO_Samod_it_1.owl#Thing"/>
    </owl:NamedIndividual>
    


    <!-- https://github.com/matteo-guenci/MiTO/blob/main/MiTO_Ontology/MiTO_Samod_it_1.owl#Theory1 -->

    <owl:NamedIndividual rdf:about="https://github.com/matteo-guenci/MiTO/blob/main/MiTO_Ontology/MiTO_Samod_it_1.owl#Theory1">
        <rdf:type rdf:resource="https://github.com/matteo-guenci/MiTO/blob/main/MiTO_Ontology/MiTO_Samod_it_1.owl#Thing"/>
    </owl:NamedIndividual>
</rdf:RDF>



<!-- Generated by the OWL API (version 4.5.25.2023-02-15T19:15:49Z) https://github.com/owlcs/owlapi -->

